cp, extraction works until here

src/riot/x509/X509.BasicFields.RelativeDistinguishedName.fst
@@ -8,7 +8,6 @@ open ASN1.Low
 open X509.Base
 
 open FStar.Integers
-module B32 = FStar.Bytes
 
 #set-options "--z3rlimit 32 --fuel 0 --ifuel 0"
 
@@ -37,16 +36,6 @@ module B32 = FStar.Bytes
  *         bmpString               BMPString (SIZE (1..MAX)) }
  *)
 
-(* TODO: Correct this once other string types are implemented *)
-let x509_RDN_attribute_oid: Type
-= oid: datatype_of_asn1_type OID
-       { oid == OID_AT_CN \/
-         oid == OID_AT_COUNTRY \/
-         oid == OID_AT_ORGANIZATION }
-
-let directory_string_type : Type
-= a: asn1_tag_t { a == IA5_STRING \/ a == PRINTABLE_STRING }
-
 // let directory_string_value
 //   (t: directory_string_type)
 // = datatype_of_asn1_type t
@@ -74,71 +63,18 @@ let directory_string_type : Type
 //   | RDN_ORGANIZATION t _ -> t
 // #pop-options
 
-inline_for_extraction
-let x509_RDN_payload_t
-  (oid: x509_RDN_attribute_oid)
-  (t: directory_string_type)
-  (lb: asn1_int32)
-  (ub: asn1_value_int32_of_type t { lb <= ub })
-= (oid `envelop_OID_with_t`
-  (asn1_string_with_character_bound_t t (count_character t) lb ub))
-
-let parse_RDN_payload
-  (oid: x509_RDN_attribute_oid)
-  (t: directory_string_type)
-  (lb: asn1_int32)
-  (ub: asn1_value_int32_of_type t { lb <= ub })
-: parser _ (x509_RDN_payload_t oid t lb ub)
-= (oid `parse_envelop_OID_with`
-   serialize_asn1_character_string_with_character_bound t lb ub)
-
-let serialize_RDN_payload
-  (oid: x509_RDN_attribute_oid)
-  (t: directory_string_type)
-  (lb: asn1_int32)
-  (ub: asn1_value_int32_of_type t { lb <= ub })
-: serializer (parse_RDN_payload oid t lb ub)
-= (oid `serialize_envelop_OID_with`
-   serialize_asn1_character_string_with_character_bound t lb ub)
-
-noextract inline_for_extraction
-let serialize32_RDN_payload_backwards
-  (oid: x509_RDN_attribute_oid)
-  (t: directory_string_type)
-  (lb: asn1_int32)
-  (ub: asn1_value_int32_of_type t { lb <= ub })
-: serializer32_backwards (serialize_RDN_payload oid t lb ub)
+let serialize32_RDN_payload_backwards oid t lb ub
 = (oid `serialize32_envelop_OID_with_backwards`
    serialize32_asn1_character_string_with_character_bound_backwards t lb ub)
 
-inline_for_extraction
-let x509_RDN_t
-  (oid: x509_RDN_attribute_oid)
-  (t: directory_string_type)
-  (lb: asn1_int32)
-  (ub: asn1_value_int32_of_type t { lb <= ub })
-= SET `inbound_envelop_tag_with_value_of`
-  (**) (SEQUENCE `serialize_asn1_envelop_tag_with_TLV`
-       (**) (serialize_RDN_payload oid t lb ub))
-
-let parse_RDN
-  (oid: x509_RDN_attribute_oid)
-  (t: directory_string_type)
-  (lb: asn1_int32)
-  (ub: asn1_value_int32_of_type t { lb <= ub })
-: parser (parse_asn1_envelop_tag_with_TLV_kind (SET)) (x509_RDN_t oid t lb ub)
+let parse_RDN oid t lb ub
 = (x509_RDN_t oid t lb ub)
   `coerce_parser`
   (SET `parse_asn1_envelop_tag_with_TLV`
   (**) (SEQUENCE `serialize_asn1_envelop_tag_with_TLV`
        (**) (serialize_RDN_payload oid t lb ub)))
 
-let serialize_RDN
-  (oid: x509_RDN_attribute_oid)
-  (t: directory_string_type)
-  (lb: asn1_int32)
-  (ub: asn1_value_int32_of_type t { lb <= ub })
-: serializer (parse_RDN oid t lb ub)
+let serialize_RDN oid t lb ub
 = coerce_parser_serializer
     (parse_RDN oid t lb ub)
     (SET `serialize_asn1_envelop_tag_with_TLV`
@@ -146,70 +82,7 @@ let serialize_RDN
        (**) (serialize_RDN_payload oid t lb ub)))
     ()
 
-let valid_RDN_ingredients
-  (oid: x509_RDN_attribute_oid)
-  (t: directory_string_type)
-  (s: datatype_of_asn1_type t)
-: Type0
-= (length_of_asn1_primitive_TLV #OID oid +
-   length_of_asn1_primitive_TLV #t s)
-  <= asn1_value_length_max_of_type SEQUENCE /\
-  (SEQUENCE `length_of_TLV`
-  (**) (length_of_asn1_primitive_TLV #OID oid +
-        length_of_asn1_primitive_TLV #t s))
-  <= asn1_value_length_max_of_type SET /\
-  (SET `length_of_TLV`
-  (**) (SEQUENCE `length_of_TLV`
-  (**) (length_of_asn1_primitive_TLV #OID oid +
-        length_of_asn1_primitive_TLV #t s)))
-  <= asn1_TLV_length_max_of_type SET
-
-let length_of_RDN
-  (oid: x509_RDN_attribute_oid)
-  (t: directory_string_type)
-  (s: datatype_of_asn1_type t
-      { valid_RDN_ingredients oid t s })
-: GTot (asn1_TLV_length_of_type SET)
-= (SET `length_of_TLV`
-  (**) (SEQUENCE `length_of_TLV`
-       (**) (length_of_asn1_primitive_TLV #OID oid +
-             length_of_asn1_primitive_TLV #t s)))
-
-noextract inline_for_extraction
-let len_of_RDN
-  (oid: x509_RDN_attribute_oid)
-  (t: directory_string_type)
-  (s: datatype_of_asn1_type t
-      { valid_RDN_ingredients oid t s })
-: Tot (len: asn1_TLV_int32_of_type SET
-            { v len == length_of_RDN oid t s })
-= (SET `len_of_TLV`
-  (**) (SEQUENCE `len_of_TLV`
-       (**) (len_of_asn1_primitive_TLV #OID oid +
-             len_of_asn1_primitive_TLV #t s)))
-
-let lemma_serialize_RDN_unfold
-  (oid: x509_RDN_attribute_oid)
-  (t: directory_string_type)
-  (lb: asn1_int32)
-  (ub: asn1_value_int32_of_type t { lb <= ub })
-  (x: x509_RDN_t oid t lb ub)
-: Lemma ( predicate_serialize_asn1_envelop_tag_with_TLV_unfold
-            (SET)
-            (**) (SEQUENCE `serialize_asn1_envelop_tag_with_TLV`
-                 (**) (oid `serialize_envelop_OID_with`
-                 (**)  serialize_asn1_character_string_with_character_bound t lb ub))
-            (x) /\
-          predicate_serialize_asn1_envelop_tag_with_TLV_unfold
-            (SEQUENCE)
-            (**) (oid `serialize_envelop_OID_with`
-            (**)  serialize_asn1_character_string_with_character_bound t lb ub)
-            (x) /\
-          predicate_serialize_envelop_OID_with_unfold
-            (oid)
-            (serialize_asn1_character_string_with_character_bound t lb ub)
-            (x)
-            )
+let lemma_serialize_RDN_unfold oid t lb ub x
 = lemma_serialize_asn1_envelop_tag_with_TLV_unfold
     (SET)
     (**) (SEQUENCE `serialize_asn1_envelop_tag_with_TLV`
@@ -226,28 +99,7 @@ let lemma_serialize_RDN_unfold
     (serialize_asn1_character_string_with_character_bound t lb ub)
     (x)
 
-let lemma_serialize_RDN_size
-  (oid: x509_RDN_attribute_oid)
-  (t: directory_string_type)
-  (lb: asn1_int32)
-  (ub: asn1_value_int32_of_type t { lb <= ub })
-  (x: x509_RDN_t oid t lb ub)
-: Lemma ( predicate_serialize_asn1_envelop_tag_with_TLV_size
-            (SET)
-            (**) (SEQUENCE `serialize_asn1_envelop_tag_with_TLV`
-                 (**) (oid `serialize_envelop_OID_with`
-                 (**)  serialize_asn1_character_string_with_character_bound t lb ub))
-            (x) /\
-          predicate_serialize_asn1_envelop_tag_with_TLV_size
-            (SEQUENCE)
-            (**) (oid `serialize_envelop_OID_with`
-            (**)  serialize_asn1_character_string_with_character_bound t lb ub)
-            (x) /\
-          predicate_serialize_envelop_OID_with_size
-            (oid)
-            (serialize_asn1_character_string_with_character_bound t lb ub)
-            (x)
-            )
+let lemma_serialize_RDN_size oid t lb ub x
 = lemma_serialize_asn1_envelop_tag_with_TLV_size
     (SET)
     (**) (SEQUENCE `serialize_asn1_envelop_tag_with_TLV`
@@ -264,72 +116,7 @@ let lemma_serialize_RDN_size
     (serialize_asn1_character_string_with_character_bound t lb ub)
     (x)
 
-let lemma_serialize_RDN_size_exact
-  (oid: x509_RDN_attribute_oid)
-  (t: directory_string_type)
-  (lb: asn1_int32)
-  (ub: asn1_value_int32_of_type t { lb <= ub })
-  (x: x509_RDN_t oid t lb ub)
-: Lemma (
-  let x': SEQUENCE `inbound_envelop_tag_with_value_of`
-          (oid `serialize_envelop_OID_with`
-           serialize_asn1_character_string_with_character_bound t lb ub)
-         = (   (coerce_envelop
-                 (SET)
-                 (SEQUENCE)
-                 (oid `serialize_envelop_OID_with`
-                  serialize_asn1_character_string_with_character_bound t lb ub)
-                 (x))) in
-  let s = snd x' in
-  let _ = lemma_serialize_RDN_size oid t lb ub x in
-  // let _ = lemma_serialize_asn1_oid_TLV_of_size oid oid in
-  length_of_opaque_serialization (serialize_RDN oid t lb ub) x <= asn1_TLV_length_max_of_type SET /\
-  length_of_opaque_serialization
-    (SEQUENCE `serialize_asn1_envelop_tag_with_TLV`
-    (**) (oid `serialize_envelop_OID_with`
-    (**)  serialize_asn1_character_string_with_character_bound t lb ub))
-    (x)
-  <= asn1_TLV_length_max_of_type SEQUENCE /\
-  // let y = x <: x509_RDN_t oid lb ub t in
-  // asn1_value_length_inbound_of_type SET
-  // (length_of_opaque_serialization
-  //   (SEQUENCE `serialize_asn1_envelop_tag_with_TLV`
-  //   (**) (oid `serialize_envelop_OID_with`
-  //   (**)  serialize_asn1_character_string_with_character_bound t lb ub))
-  //   (x)) /\
-  // (length_of_asn1_primitive_TLV #OID oid +
-  //  length_of_asn1_primitive_TLV #t s)
-  length_of_opaque_serialization
-    (oid `serialize_envelop_OID_with`
-     serialize_asn1_character_string_with_character_bound t lb ub)
-    (x)
-  <= asn1_value_length_max_of_type SEQUENCE /\
-  length_of_opaque_serialization
-    (oid `serialize_envelop_OID_with`
-     serialize_asn1_character_string_with_character_bound t lb ub)
-    (x)
-  == length_of_envelop_OID_with
-            (oid)
-            (serialize_asn1_character_string_with_character_bound t lb ub)
-            (s) /\
-  length_of_opaque_serialization (serialize_asn1_character_string_with_character_bound t lb ub) (s)
-  == length_of_asn1_primitive_TLV #t s /\
-  length_of_opaque_serialization (serialize_asn1_oid_TLV_of oid) oid
-  == length_of_asn1_primitive_TLV #OID oid /\
-  length_of_opaque_serialization
-    (oid `serialize_envelop_OID_with`
-     serialize_asn1_character_string_with_character_bound t lb ub)
-    (x)
-  == (length_of_asn1_primitive_TLV #OID oid +
-      length_of_asn1_primitive_TLV #t s) /\
-  (SEQUENCE `length_of_TLV`
-        (**) (length_of_asn1_primitive_TLV #OID oid +
-              length_of_asn1_primitive_TLV #t s))
-        <= asn1_TLV_length_max_of_type SEQUENCE /\
-  length_of_opaque_serialization (serialize_RDN oid t lb ub) x
-  == length_of_RDN oid t s /\
-  True
-)
+let lemma_serialize_RDN_size_exact oid t lb ub x
 = lemma_serialize_RDN_unfold oid t lb ub x;
   lemma_serialize_RDN_size   oid t lb ub x;
   lemma_serialize_envelop_OID_with_size
@@ -339,12 +126,9 @@ let lemma_serialize_RDN_size_exact
   // lemma_serialize_asn1_oid_TLV_of_size oid oid
 ()
 
-noextract inline_for_extraction
-let serialize32_RDN_backwards
-  (oid: x509_RDN_attribute_oid)
-  (t: directory_string_type)
-  (lb: asn1_int32)
-  (ub: asn1_value_int32_of_type t { lb <= ub })
+#push-options "--ifuel 1"
+
+let serialize32_RDN_backwards oid t lb ub
 = coerce_serializer32_backwards
   (* s2  *) (serialize_RDN oid t lb ub)
   (* s32 *) (SET `serialize32_asn1_envelop_tag_with_TLV_backwards`
@@ -354,81 +138,7 @@ let serialize32_RDN_backwards
 
 (*  *)
 
-type x520_attribute_t =
-| COUNTRY
-| ORGANIZATION
-// | ORGANIZATIONAL_UNIT
-// | DISTINGUISHED_NAME_QUALIFIER
-// | STATE_OR_PROVINCE_NAME
-| COMMON_NAME
-// | SERIAL_NUMBER
-
-#push-options "--ifuel 1"
-let x520_attribute_lb
-  (t: x520_attribute_t)
-: Tot (asn1_int32)
-= match t with
-  | COUNTRY      -> 2ul
-  | ORGANIZATION -> 1ul
-  | COMMON_NAME  -> 1ul
-
-let x520_attribute_ub
-  (t: x520_attribute_t)
-: Tot (len: asn1_int32 { len >= x520_attribute_lb t })
-= match t with
-  | COUNTRY      -> 2ul
-  | ORGANIZATION -> 64ul
-  | COMMON_NAME  -> 32768ul
-
-inline_for_extraction
-let x520_attribute_oid
-  (t: x520_attribute_t)
-: Tot (datatype_of_asn1_type OID)
-= match t with
-  | COUNTRY      -> OID_AT_COUNTRY
-  | ORGANIZATION -> OID_AT_ORGANIZATION
-  | COMMON_NAME  -> OID_AT_CN
-
-inline_for_extraction
-let x509_RDN_x520_attribute_t
-  (t: x520_attribute_t)
-  (string_t: directory_string_type { ((t == COUNTRY) ==> (string_t == PRINTABLE_STRING)) })
-= x509_RDN_t
-    (x520_attribute_oid t)
-    (string_t)
-    (x520_attribute_lb t)
-    (x520_attribute_ub t)
-
-noextract inline_for_extraction
-let x509_RDN_x520_attribute_string_t
-  (t: x520_attribute_t)
-  (string_t: directory_string_type { ((t == COUNTRY) ==> (string_t == PRINTABLE_STRING)) })
-// = get_parser_type (parse_asn1_character_string_with_character_bound string_t (x520_attribute_lb t) (x520_attribute_ub t))
-= asn1_string_with_character_bound_t
-    (string_t)
-    (count_character string_t)
-    (x520_attribute_lb t)
-    (x520_attribute_ub t)
-
-let lemma_RDN_x520_attribute_size
-  (#t: x520_attribute_t)
-  (#string_t: directory_string_type { ((t == COUNTRY) ==> (string_t == PRINTABLE_STRING)) })
-  (s: x509_RDN_x520_attribute_string_t t string_t)
-: Lemma (
-  asn1_value_length_inbound_of_type
-    (string_t)
-    (length_of_opaque_serialization (serialize_asn1_TLV_of_type string_t) s) /\
-  asn1_value_length_inbound_of_type
-    (SEQUENCE)
-    (length_of_opaque_serialization ((x520_attribute_oid t) `serialize_envelop_OID_with`
-                                     (serialize_asn1_TLV_of_type string_t))
-                                    ((x520_attribute_oid t), s)) /\
-  (serialize_asn1_character_string_with_character_bound
-      (string_t)
-      (x520_attribute_lb t)
-      (x520_attribute_ub t)) `serialize` s
-  == serialize_asn1_TLV_of_type string_t `serialize` s
-)
+let lemma_RDN_x520_attribute_size #t #string_t s
 = lemma_serialize_character_string_size string_t s;
   lemma_serialize_asn1_oid_TLV_of_size (x520_attribute_oid t) (x520_attribute_oid t);
   lemma_serialize_envelop_OID_with_size
@@ -436,87 +146,25 @@ let lemma_RDN_x520_attribute_size
     (serialize_asn1_TLV_of_type string_t)
     ((x520_attribute_oid t), s)
 
-let parse_RDN_x520_attribute
-  (t: x520_attribute_t)
-  (string_t: directory_string_type { ((t == COUNTRY) ==> (string_t == PRINTABLE_STRING)) })
-: parser (parse_asn1_envelop_tag_with_TLV_kind (SET)) (x509_RDN_x520_attribute_t t string_t)
+let parse_RDN_x520_attribute t string_t
 = (x509_RDN_x520_attribute_t t string_t)
   `coerce_parser`
   (parse_RDN (x520_attribute_oid t) (string_t) (x520_attribute_lb t) (x520_attribute_ub t))
 
-let serialize_RDN_x520_attribute
-  (t: x520_attribute_t)
-  (string_t: directory_string_type { ((t == COUNTRY) ==> (string_t == PRINTABLE_STRING)) })
-: serializer (parse_RDN_x520_attribute t string_t)
+let serialize_RDN_x520_attribute t string_t
 = coerce_parser_serializer
     (parse_RDN_x520_attribute t string_t)
     (serialize_RDN (x520_attribute_oid t) (string_t) (x520_attribute_lb t) (x520_attribute_ub t))
     ()
 
-let length_of_RDN_x520_attribute
-  (#t: x520_attribute_t)
-  (#string_t: directory_string_type { ((t == COUNTRY) ==> (string_t == PRINTABLE_STRING)) })
-  (s: x509_RDN_x520_attribute_string_t t string_t)
-: GTot (asn1_TLV_length_of_type SET)
-= length_of_RDN
-    (x520_attribute_oid t)
-    (string_t)
-    (s)
-
-noextract inline_for_extraction
-let len_of_RDN_x520_attribute
-  (#t: x520_attribute_t)
-  (#string_t: directory_string_type { ((t == COUNTRY) ==> (string_t == PRINTABLE_STRING)) })
-  (s: x509_RDN_x520_attribute_string_t t string_t)
-: Tot (len: asn1_TLV_int32_of_type SET
-            { v len == length_of_RDN_x520_attribute s })
-= len_of_RDN
-    (x520_attribute_oid t)
-    (string_t)
-    (s)
-
-noextract inline_for_extraction
-let get_RDN_x520_attribute_string
-  (#t: x520_attribute_t)
-  (#string_t: directory_string_type { ((t == COUNTRY) ==> (string_t == PRINTABLE_STRING)) })
-  (x: x509_RDN_x520_attribute_t t string_t)
-: Tot (x509_RDN_x520_attribute_string_t t string_t)
-= snd (coerce_envelop
-        (SET)
-        (SEQUENCE)
-        ((x520_attribute_oid t) `serialize_envelop_OID_with`
-          serialize_asn1_character_string_with_character_bound string_t (x520_attribute_lb t) (x520_attribute_ub t))
-        (x))
-
-let lemma_serialize_RDN_x520_attribute_unfold
-  (#t: x520_attribute_t)
-  (#string_t: directory_string_type { ((t == COUNTRY) ==> (string_t == PRINTABLE_STRING)) })
-  (x: x509_RDN_x520_attribute_t t string_t)
-= lemma_serialize_RDN_unfold (x520_attribute_oid t) (string_t) (x520_attribute_lb t) (x520_attribute_ub t) x
-
-let lemma_serialize_RDN_x520_attribute_size
-  (#t: x520_attribute_t)
-  (#string_t: directory_string_type { ((t == COUNTRY) ==> (string_t == PRINTABLE_STRING)) })
-  (x: x509_RDN_x520_attribute_t t string_t)
-= lemma_serialize_RDN_size (x520_attribute_oid t) (string_t) (x520_attribute_lb t) (x520_attribute_ub t) x
 
 #push-options "--z3rlimit 64"
-let lemma_serialize_RDN_x520_attribute_size_exact
-  (#t: x520_attribute_t)
-  (#string_t: directory_string_type { ((t == COUNTRY) ==> (string_t == PRINTABLE_STRING)) })
-  (x: x509_RDN_x520_attribute_t t string_t)
-: Lemma (
-  length_of_opaque_serialization (serialize_RDN_x520_attribute _ _) x
-  == length_of_RDN_x520_attribute (get_RDN_x520_attribute_string x)
-)
+let lemma_serialize_RDN_x520_attribute_size_exact #t #string_t x
 = lemma_serialize_RDN_size_exact (x520_attribute_oid t) (string_t) (x520_attribute_lb t) (x520_attribute_ub t) x
 #pop-options
 
-noextract inline_for_extraction
-let serialize32_RDN_x520_attribute_backwards
-  (t: x520_attribute_t)
-  (string_t: directory_string_type { ((t == COUNTRY) ==> (string_t == PRINTABLE_STRING)) })
-: serializer32_backwards (serialize_RDN_x520_attribute t string_t)
+#push-options "--z3rlimit 96"
+let serialize32_RDN_x520_attribute_backwards t string_t
 = coerce_serializer32_backwards
     (serialize_RDN_x520_attribute t string_t)
     (serialize32_RDN_backwards (x520_attribute_oid t) (string_t) (x520_attribute_lb t) (x520_attribute_ub t))
@@ -530,57 +178,6 @@ let serialize32_RDN_x520_attribute_backwards
 //   (|3ul, B32.hide (Seq.createL [0x10uy; 0x11uy; 0x12uy])|) <: datatype_of_asn1_type IA5_STRING
 
 // #push-options "--max_fuel 4 --max_ifuel 4"
-noextract inline_for_extraction
-let asn1_get_character_string
-  (#string_t: character_string_type)
-  (len: asn1_value_int32_of_type string_t)
-  (s32: character_string_lbytes32 string_t len)
-: Tot (datatype_of_asn1_type string_t)
-= (|len, s32|) <: character_string_t string_t
-
-noextract inline_for_extraction
-let x509_get_RDN_x520_attribute_string
-  (#t: x520_attribute_t)
-  (#string_t: directory_string_type { ((t == COUNTRY) ==> (string_t == PRINTABLE_STRING)) })
-  (x: parse_filter_refine (filter_asn1_string_with_character_bound string_t
-                            (count_character string_t)
-                            (x520_attribute_lb t)
-                            (x520_attribute_ub t)))
-: Tot (x509_RDN_x520_attribute_string_t t string_t)
-= x
-
-#push-options "--z3rlimit 96"
-noextract inline_for_extraction
-let x509_get_RDN_x520_attribute
-  (#t: x520_attribute_t)
-  (#string_t: directory_string_type { ((t == COUNTRY) ==> (string_t == PRINTABLE_STRING)) })
-  (x: x509_RDN_x520_attribute_string_t t string_t)
-: Tot (x509_RDN_x520_attribute_t t string_t)
-=
-  [@inline_let]
-  let attr: (x520_attribute_oid t) `envelop_OID_with_t`
-            (x509_RDN_x520_attribute_string_t t string_t) = (
-      x520_attribute_oid t,
-      x
-  ) in
-  (* Prf *) lemma_serialize_asn1_oid_TLV_of_size (x520_attribute_oid t) (x520_attribute_oid t);
-  (* Prf *) lemma_serialize_character_string_size string_t x;
-  (* Prf *) lemma_serialize_envelop_OID_with_size
-              (x520_attribute_oid t)
-              (serialize_asn1_character_string_with_character_bound
-                (string_t)
-                (x520_attribute_lb t)
-                (x520_attribute_ub t))
-              (attr);
-  (* Prf *) lemma_serialize_asn1_sequence_TLV_size
-              ((x520_attribute_oid t) `serialize_envelop_OID_with`
-               (serialize_asn1_character_string_with_character_bound
-                (string_t)
-                (x520_attribute_lb t)
-                (x520_attribute_ub t)))
-              (attr);
-(* return *) (attr)
-#pop-options
 
 (*
  *   Standard sets of attributes have been defined in the X.500 series of
