src/riot/x509/X509.BasicFields.RelativeDistinguishedName.fsti
@@ -1,0 +1,593 @@
+module X509.BasicFields.RelativeDistinguishedName
+
+open ASN1.Spec
+open ASN1.Low
+
+open X509.Base
+
+open FStar.Integers
+
+#set-options "--z3rlimit 32 --fuel 0 --ifuel 0"
+
+(*
+ *   Name ::= CHOICE { -- only one possibility for now --
+ *     rdnSequence  RDNSequence }
+ *
+ *   RDNSequence ::= SEQUENCE OF RelativeDistinguishedName
+ *
+ *   RelativeDistinguishedName ::=
+ *     SET SIZE (1..MAX) OF AttributeTypeAndValue
+ *
+ *   AttributeTypeAndValue ::= SEQUENCE {
+ *     type     AttributeType,
+ *     value    AttributeValue }
+ *
+ *   AttributeType ::= OBJECT IDENTIFIER
+ *
+ *   AttributeValue ::= ANY -- DEFINED BY AttributeType
+ *
+ *   DirectoryString ::= CHOICE {
+ *         teletexString           TeletexString (SIZE (1..MAX)),
+ *         printableString         PrintableString (SIZE (1..MAX)),
+ *         universalString         UniversalString (SIZE (1..MAX)),
+ *         utf8String              UTF8String (SIZE (1..MAX)),
+ *         bmpString               BMPString (SIZE (1..MAX)) }
+ *)
+
+(* TODO: Correct this once other string types are implemented *)
+let x509_RDN_attribute_oid: Type
+= oid: datatype_of_asn1_type OID
+       { oid == OID_AT_CN \/
+         oid == OID_AT_COUNTRY \/
+         oid == OID_AT_ORGANIZATION }
+
+unfold
+let directory_string_type : Type
+= a: asn1_tag_t { a == IA5_STRING \/ a == PRINTABLE_STRING }
+
+// let directory_string_value
+//   (t: directory_string_type)
+// = datatype_of_asn1_type t
+
+// type x509_RDN_payload_t =
+// | RDN_CN          : t: directory_string_type -> directory_string_value t -> x509_RDN_payload_t
+// | RDN_COUNTRY     : t: directory_string_type -> directory_string_value t -> x509_RDN_payload_t
+// | RDN_ORGANIZATION: t: directory_string_type -> directory_string_value t -> x509_RDN_payload_t
+
+// #push-options "--fuel 0 --ifuel 1"
+// let oid_of_RDN
+//   (rdn: x509_RDN_payload_t)
+// : Tot (x509_RDN_attribute_oid)
+// = match rdn with
+//   | RDN_CN           _ _ -> OID_AT_CN
+//   | RDN_COUNTRY      _ _ -> OID_AT_COUNTRY
+//   | RDN_ORGANIZATION _ _ -> OID_AT_ORGANIZATION
+
+// let asn1_type_of_RDN
+//   (rdn: x509_RDN_payload_t)
+// : Tot (directory_string_type)
+// = match rdn with
+//   | RDN_CN           t _ -> t
+//   | RDN_COUNTRY      t _ -> t
+//   | RDN_ORGANIZATION t _ -> t
+// #pop-options
+
+unfold noextract
+let x509_RDN_payload_t
+  (oid: x509_RDN_attribute_oid)
+  (t: directory_string_type)
+  (lb: asn1_int32)
+  (ub: asn1_value_int32_of_type t { lb <= ub })
+= (oid `envelop_OID_with_t`
+  (asn1_string_with_character_bound_t t (count_character t) lb ub))
+
+let parse_RDN_payload
+  (oid: x509_RDN_attribute_oid)
+  (t: directory_string_type)
+  (lb: asn1_int32)
+  (ub: asn1_value_int32_of_type t { lb <= ub })
+: parser _ (x509_RDN_payload_t oid t lb ub)
+= (oid `parse_envelop_OID_with`
+   serialize_asn1_character_string_with_character_bound t lb ub)
+
+let serialize_RDN_payload
+  (oid: x509_RDN_attribute_oid)
+  (t: directory_string_type)
+  (lb: asn1_int32)
+  (ub: asn1_value_int32_of_type t { lb <= ub })
+: serializer (parse_RDN_payload oid t lb ub)
+= (oid `serialize_envelop_OID_with`
+   serialize_asn1_character_string_with_character_bound t lb ub)
+
+noextract inline_for_extraction
+val serialize32_RDN_payload_backwards
+  (oid: x509_RDN_attribute_oid)
+  (t: directory_string_type)
+  (lb: asn1_int32)
+  (ub: asn1_value_int32_of_type t { lb <= ub })
+: serializer32_backwards (serialize_RDN_payload oid t lb ub)
+
+unfold noextract
+let x509_RDN_t
+  (oid: x509_RDN_attribute_oid)
+  (t: directory_string_type)
+  (lb: asn1_int32)
+  (ub: asn1_value_int32_of_type t { lb <= ub })
+= SET `inbound_envelop_tag_with_value_of`
+  (**) (SEQUENCE `serialize_asn1_envelop_tag_with_TLV`
+       (**) (serialize_RDN_payload oid t lb ub))
+
+noextract
+val parse_RDN
+  (oid: x509_RDN_attribute_oid)
+  (t: directory_string_type)
+  (lb: asn1_int32)
+  (ub: asn1_value_int32_of_type t { lb <= ub })
+: parser (parse_asn1_envelop_tag_with_TLV_kind (SET)) (x509_RDN_t oid t lb ub)
+
+noextract
+val serialize_RDN
+  (oid: x509_RDN_attribute_oid)
+  (t: directory_string_type)
+  (lb: asn1_int32)
+  (ub: asn1_value_int32_of_type t { lb <= ub })
+: serializer (parse_RDN oid t lb ub)
+
+unfold
+let valid_RDN_ingredients
+  (oid: x509_RDN_attribute_oid)
+  (t: directory_string_type)
+  (s: datatype_of_asn1_type t)
+: Type0
+= (length_of_asn1_primitive_TLV #OID oid +
+   length_of_asn1_primitive_TLV #t s)
+  <= asn1_value_length_max_of_type SEQUENCE /\
+  (SEQUENCE `length_of_TLV`
+  (**) (length_of_asn1_primitive_TLV #OID oid +
+        length_of_asn1_primitive_TLV #t s))
+  <= asn1_value_length_max_of_type SET /\
+  (SET `length_of_TLV`
+  (**) (SEQUENCE `length_of_TLV`
+  (**) (length_of_asn1_primitive_TLV #OID oid +
+        length_of_asn1_primitive_TLV #t s)))
+  <= asn1_TLV_length_max_of_type SET
+
+unfold
+let length_of_RDN
+  (oid: x509_RDN_attribute_oid)
+  (t: directory_string_type)
+  (s: datatype_of_asn1_type t
+      { valid_RDN_ingredients oid t s })
+: GTot (asn1_TLV_length_of_type SET)
+= (SET `length_of_TLV`
+  (**) (SEQUENCE `length_of_TLV`
+       (**) (length_of_asn1_primitive_TLV #OID oid +
+             length_of_asn1_primitive_TLV #t s)))
+
+unfold noextract
+let len_of_RDN
+  (oid: x509_RDN_attribute_oid)
+  (t: directory_string_type)
+  (s: datatype_of_asn1_type t
+      { valid_RDN_ingredients oid t s })
+: Tot (len: asn1_TLV_int32_of_type SET
+            { v len == length_of_RDN oid t s })
+= (SET `len_of_TLV`
+  (**) (SEQUENCE `len_of_TLV`
+       (**) (len_of_asn1_primitive_TLV #OID oid +
+             len_of_asn1_primitive_TLV #t s)))
+
+val lemma_serialize_RDN_unfold
+  (oid: x509_RDN_attribute_oid)
+  (t: directory_string_type)
+  (lb: asn1_int32)
+  (ub: asn1_value_int32_of_type t { lb <= ub })
+  (x: x509_RDN_t oid t lb ub)
+: Lemma ( predicate_serialize_asn1_envelop_tag_with_TLV_unfold
+            (SET)
+            (**) (SEQUENCE `serialize_asn1_envelop_tag_with_TLV`
+                 (**) (oid `serialize_envelop_OID_with`
+                 (**)  serialize_asn1_character_string_with_character_bound t lb ub))
+            (x) /\
+          predicate_serialize_asn1_envelop_tag_with_TLV_unfold
+            (SEQUENCE)
+            (**) (oid `serialize_envelop_OID_with`
+            (**)  serialize_asn1_character_string_with_character_bound t lb ub)
+            (x) /\
+          predicate_serialize_envelop_OID_with_unfold
+            (oid)
+            (serialize_asn1_character_string_with_character_bound t lb ub)
+            (x)
+            )
+
+val lemma_serialize_RDN_size
+  (oid: x509_RDN_attribute_oid)
+  (t: directory_string_type)
+  (lb: asn1_int32)
+  (ub: asn1_value_int32_of_type t { lb <= ub })
+  (x: x509_RDN_t oid t lb ub)
+: Lemma ( predicate_serialize_asn1_envelop_tag_with_TLV_size
+            (SET)
+            (**) (SEQUENCE `serialize_asn1_envelop_tag_with_TLV`
+                 (**) (oid `serialize_envelop_OID_with`
+                 (**)  serialize_asn1_character_string_with_character_bound t lb ub))
+            (x) /\
+          predicate_serialize_asn1_envelop_tag_with_TLV_size
+            (SEQUENCE)
+            (**) (oid `serialize_envelop_OID_with`
+            (**)  serialize_asn1_character_string_with_character_bound t lb ub)
+            (x) /\
+          predicate_serialize_envelop_OID_with_size
+            (oid)
+            (serialize_asn1_character_string_with_character_bound t lb ub)
+            (x)
+            )
+
+val lemma_serialize_RDN_size_exact
+  (oid: x509_RDN_attribute_oid)
+  (t: directory_string_type)
+  (lb: asn1_int32)
+  (ub: asn1_value_int32_of_type t { lb <= ub })
+  (x: x509_RDN_t oid t lb ub)
+: Lemma (
+  let x': SEQUENCE `inbound_envelop_tag_with_value_of`
+          (oid `serialize_envelop_OID_with`
+           serialize_asn1_character_string_with_character_bound t lb ub)
+         = (   (coerce_envelop
+                 (SET)
+                 (SEQUENCE)
+                 (oid `serialize_envelop_OID_with`
+                  serialize_asn1_character_string_with_character_bound t lb ub)
+                 (x))) in
+  let s = snd x' in
+  let _ = lemma_serialize_RDN_size oid t lb ub x in
+  // let _ = lemma_serialize_asn1_oid_TLV_of_size oid oid in
+  length_of_opaque_serialization (serialize_RDN oid t lb ub) x <= asn1_TLV_length_max_of_type SET /\
+  length_of_opaque_serialization
+    (SEQUENCE `serialize_asn1_envelop_tag_with_TLV`
+    (**) (oid `serialize_envelop_OID_with`
+    (**)  serialize_asn1_character_string_with_character_bound t lb ub))
+    (x)
+  <= asn1_TLV_length_max_of_type SEQUENCE /\
+  // let y = x <: x509_RDN_t oid lb ub t in
+  // asn1_value_length_inbound_of_type SET
+  // (length_of_opaque_serialization
+  //   (SEQUENCE `serialize_asn1_envelop_tag_with_TLV`
+  //   (**) (oid `serialize_envelop_OID_with`
+  //   (**)  serialize_asn1_character_string_with_character_bound t lb ub))
+  //   (x)) /\
+  // (length_of_asn1_primitive_TLV #OID oid +
+  //  length_of_asn1_primitive_TLV #t s)
+  length_of_opaque_serialization
+    (oid `serialize_envelop_OID_with`
+     serialize_asn1_character_string_with_character_bound t lb ub)
+    (x)
+  <= asn1_value_length_max_of_type SEQUENCE /\
+  length_of_opaque_serialization
+    (oid `serialize_envelop_OID_with`
+     serialize_asn1_character_string_with_character_bound t lb ub)
+    (x)
+  == length_of_envelop_OID_with
+            (oid)
+            (serialize_asn1_character_string_with_character_bound t lb ub)
+            (s) /\
+  length_of_opaque_serialization (serialize_asn1_character_string_with_character_bound t lb ub) (s)
+  == length_of_asn1_primitive_TLV #t s /\
+  length_of_opaque_serialization (serialize_asn1_oid_TLV_of oid) oid
+  == length_of_asn1_primitive_TLV #OID oid /\
+  length_of_opaque_serialization
+    (oid `serialize_envelop_OID_with`
+     serialize_asn1_character_string_with_character_bound t lb ub)
+    (x)
+  == (length_of_asn1_primitive_TLV #OID oid +
+      length_of_asn1_primitive_TLV #t s) /\
+  (SEQUENCE `length_of_TLV`
+        (**) (length_of_asn1_primitive_TLV #OID oid +
+              length_of_asn1_primitive_TLV #t s))
+        <= asn1_TLV_length_max_of_type SEQUENCE /\
+  length_of_opaque_serialization (serialize_RDN oid t lb ub) x
+  == length_of_RDN oid t s /\
+  True
+)
+
+noextract inline_for_extraction
+val serialize32_RDN_backwards
+  (oid: x509_RDN_attribute_oid)
+  (t: directory_string_type)
+  (lb: asn1_int32)
+  (ub: asn1_value_int32_of_type t { lb <= ub })
+: serializer32_backwards (serialize_RDN oid t lb ub)
+
+(*  *)
+
+type x520_attribute_t =
+| COUNTRY
+| ORGANIZATION
+// | ORGANIZATIONAL_UNIT
+// | DISTINGUISHED_NAME_QUALIFIER
+// | STATE_OR_PROVINCE_NAME
+| COMMON_NAME
+// | SERIAL_NUMBER
+
+#push-options "--ifuel 1"
+unfold noextract
+let x520_attribute_lb
+  (t: x520_attribute_t)
+: Tot (asn1_int32)
+= match t with
+  | COUNTRY      -> 2ul
+  | ORGANIZATION -> 1ul
+  | COMMON_NAME  -> 1ul
+
+unfold noextract
+let x520_attribute_ub
+  (t: x520_attribute_t)
+: Tot (len: asn1_int32 { len >= x520_attribute_lb t })
+= match t with
+  | COUNTRY      -> 2ul
+  | ORGANIZATION -> 64ul
+  | COMMON_NAME  -> 32768ul
+
+unfold noextract
+let x520_attribute_oid
+  (t: x520_attribute_t)
+: Tot (datatype_of_asn1_type OID)
+= match t with
+  | COUNTRY      -> OID_AT_COUNTRY
+  | ORGANIZATION -> OID_AT_ORGANIZATION
+  | COMMON_NAME  -> OID_AT_CN
+
+unfold noextract
+let x509_RDN_x520_attribute_t
+  (t: x520_attribute_t)
+  (string_t: directory_string_type { ((t == COUNTRY) ==> (string_t == PRINTABLE_STRING)) })
+= x509_RDN_t
+    (x520_attribute_oid t)
+    (string_t)
+    (x520_attribute_lb t)
+    (x520_attribute_ub t)
+
+unfold noextract
+let x509_RDN_x520_attribute_string_t
+  (t: x520_attribute_t)
+  (string_t: directory_string_type { ((t == COUNTRY) ==> (string_t == PRINTABLE_STRING)) })
+// = get_parser_type (parse_asn1_character_string_with_character_bound string_t (x520_attribute_lb t) (x520_attribute_ub t))
+= asn1_string_with_character_bound_t
+    (string_t)
+    (count_character string_t)
+    (x520_attribute_lb t)
+    (x520_attribute_ub t)
+
+val lemma_RDN_x520_attribute_size
+  (#t: x520_attribute_t)
+  (#string_t: directory_string_type { ((t == COUNTRY) ==> (string_t == PRINTABLE_STRING)) })
+  (s: x509_RDN_x520_attribute_string_t t string_t)
+: Lemma (
+  asn1_value_length_inbound_of_type
+    (string_t)
+    (length_of_opaque_serialization (serialize_asn1_TLV_of_type string_t) s) /\
+  asn1_value_length_inbound_of_type
+    (SEQUENCE)
+    (length_of_opaque_serialization ((x520_attribute_oid t) `serialize_envelop_OID_with`
+                                     (serialize_asn1_TLV_of_type string_t))
+                                    ((x520_attribute_oid t), s)) /\
+  (serialize_asn1_character_string_with_character_bound
+      (string_t)
+      (x520_attribute_lb t)
+      (x520_attribute_ub t)) `serialize` s
+  == serialize_asn1_TLV_of_type string_t `serialize` s
+)
+
+val parse_RDN_x520_attribute
+  (t: x520_attribute_t)
+  (string_t: directory_string_type { ((t == COUNTRY) ==> (string_t == PRINTABLE_STRING)) })
+: parser (parse_asn1_envelop_tag_with_TLV_kind (SET)) (x509_RDN_x520_attribute_t t string_t)
+
+noextract
+val serialize_RDN_x520_attribute
+  (t: x520_attribute_t)
+  (string_t: directory_string_type { ((t == COUNTRY) ==> (string_t == PRINTABLE_STRING)) })
+: serializer (parse_RDN_x520_attribute t string_t)
+
+unfold
+let length_of_RDN_x520_attribute
+  (#t: x520_attribute_t)
+  (#string_t: directory_string_type { ((t == COUNTRY) ==> (string_t == PRINTABLE_STRING)) })
+  (s: x509_RDN_x520_attribute_string_t t string_t)
+: GTot (asn1_TLV_length_of_type SET)
+= length_of_RDN
+    (x520_attribute_oid t)
+    (string_t)
+    (s)
+
+unfold noextract
+let len_of_RDN_x520_attribute
+  (#t: x520_attribute_t)
+  (#string_t: directory_string_type { ((t == COUNTRY) ==> (string_t == PRINTABLE_STRING)) })
+  (s: x509_RDN_x520_attribute_string_t t string_t)
+: Tot (len: asn1_TLV_int32_of_type SET
+            { v len == length_of_RDN_x520_attribute s })
+= len_of_RDN
+    (x520_attribute_oid t)
+    (string_t)
+    (s)
+
+unfold noextract
+let get_RDN_x520_attribute_string
+  (#t: x520_attribute_t)
+  (#string_t: directory_string_type { ((t == COUNTRY) ==> (string_t == PRINTABLE_STRING)) })
+  (x: x509_RDN_x520_attribute_t t string_t)
+: Tot (x509_RDN_x520_attribute_string_t t string_t)
+= snd (coerce_envelop
+        (SET)
+        (SEQUENCE)
+        ((x520_attribute_oid t) `serialize_envelop_OID_with`
+          serialize_asn1_character_string_with_character_bound string_t (x520_attribute_lb t) (x520_attribute_ub t))
+        (x))
+
+let lemma_serialize_RDN_x520_attribute_unfold
+  (#t: x520_attribute_t)
+  (#string_t: directory_string_type { ((t == COUNTRY) ==> (string_t == PRINTABLE_STRING)) })
+  (x: x509_RDN_x520_attribute_t t string_t)
+= lemma_serialize_RDN_unfold (x520_attribute_oid t) (string_t) (x520_attribute_lb t) (x520_attribute_ub t) x
+
+let lemma_serialize_RDN_x520_attribute_size
+  (#t: x520_attribute_t)
+  (#string_t: directory_string_type { ((t == COUNTRY) ==> (string_t == PRINTABLE_STRING)) })
+  (x: x509_RDN_x520_attribute_t t string_t)
+= lemma_serialize_RDN_size (x520_attribute_oid t) (string_t) (x520_attribute_lb t) (x520_attribute_ub t) x
+
+val lemma_serialize_RDN_x520_attribute_size_exact
+  (#t: x520_attribute_t)
+  (#string_t: directory_string_type { ((t == COUNTRY) ==> (string_t == PRINTABLE_STRING)) })
+  (x: x509_RDN_x520_attribute_t t string_t)
+: Lemma (
+  length_of_opaque_serialization (serialize_RDN_x520_attribute _ _) x
+  == length_of_RDN_x520_attribute (get_RDN_x520_attribute_string x)
+)
+
+noextract inline_for_extraction
+val serialize32_RDN_x520_attribute_backwards
+  (t: x520_attribute_t)
+  (string_t: directory_string_type { ((t == COUNTRY) ==> (string_t == PRINTABLE_STRING)) })
+: serializer32_backwards (serialize_RDN_x520_attribute t string_t)
+
+// #push-options "--fuel 4 --ifuel 0"
+// let _ = assert_norm (Seq.for_all valid_IA5_byte (B32.reveal (B32.hide (Seq.createL [0x10uy; 0x11uy; 0x12uy]))) )
+
+// let x: x509_RDN_x520_attribute_string_t COMMON_NAME IA5_STRING
+// = assert_norm (Seq.for_all valid_IA5_byte (B32.reveal (B32.hide (Seq.createL [0x10uy; 0x11uy; 0x12uy]))));
+//   (|3ul, B32.hide (Seq.createL [0x10uy; 0x11uy; 0x12uy])|) <: datatype_of_asn1_type IA5_STRING
+
+// #push-options "--max_fuel 4 --max_ifuel 4"
+unfold noextract
+let asn1_get_character_string
+  (#string_t: character_string_type)
+  (len: asn1_value_int32_of_type string_t)
+  (s32: character_string_lbytes32 string_t len)
+: Tot (datatype_of_asn1_type string_t)
+= (|len, s32|) <: character_string_t string_t
+
+unfold noextract
+let x509_get_RDN_x520_attribute_string
+  (#t: x520_attribute_t)
+  (#string_t: directory_string_type { ((t == COUNTRY) ==> (string_t == PRINTABLE_STRING)) })
+  (x: parse_filter_refine (filter_asn1_string_with_character_bound string_t
+                            (count_character string_t)
+                            (x520_attribute_lb t)
+                            (x520_attribute_ub t)))
+: Tot (x509_RDN_x520_attribute_string_t t string_t)
+= x
+
+#push-options "--z3rlimit 96"
+unfold noextract
+let x509_get_RDN_x520_attribute
+  (#t: x520_attribute_t)
+  (#string_t: directory_string_type { ((t == COUNTRY) ==> (string_t == PRINTABLE_STRING)) })
+  (x: x509_RDN_x520_attribute_string_t t string_t)
+: Tot (x509_RDN_x520_attribute_t t string_t)
+=
+  [@inline_let]
+  let attr: (x520_attribute_oid t) `envelop_OID_with_t`
+            (x509_RDN_x520_attribute_string_t t string_t) = (
+      x520_attribute_oid t,
+      x
+  ) in
+  (* Prf *) lemma_serialize_asn1_oid_TLV_of_size (x520_attribute_oid t) (x520_attribute_oid t);
+  (* Prf *) lemma_serialize_character_string_size string_t x;
+  (* Prf *) lemma_serialize_envelop_OID_with_size
+              (x520_attribute_oid t)
+              (serialize_asn1_character_string_with_character_bound
+                (string_t)
+                (x520_attribute_lb t)
+                (x520_attribute_ub t))
+              (attr);
+  (* Prf *) lemma_serialize_asn1_sequence_TLV_size
+              ((x520_attribute_oid t) `serialize_envelop_OID_with`
+               (serialize_asn1_character_string_with_character_bound
+                (string_t)
+                (x520_attribute_lb t)
+                (x520_attribute_ub t)))
+              (attr);
+(* return *) (attr)
+#pop-options
+
+(*
+ *   Standard sets of attributes have been defined in the X.500 series of
+ *   specifications [X.520].  Implementations of this specification MUST
+ *   be prepared to receive the following standard attribute types in
+ *   issuer and subject (Section 4.1.2.6) names:
+ *
+ *      * country,
+ *      * organization,
+ *      * organizational unit,
+ *      * distinguished name qualifier,
+ *      * state or province name,
+ *      * common name (e.g., "Susan Housley"), and
+ *      * serial number.
+ *
+ *   In addition, implementations of this specification SHOULD be prepared
+ *   to receive the following standard attribute types in issuer and
+ *   subject names:
+ *
+ *      * locality,
+ *      * title,
+ *      * surname,
+ *      * given name,
+ *      * initials,
+ *      * pseudonym, and
+ *      * generation qualifier (e.g., "Jr.", "3rd", or "IV").
+ *
+ *   The syntax and associated object identifiers (OIDs) for these
+ *   attribute types are provided in the ASN.1 modules in Appendix A.
+ *)
+
+(*
+ * -- Upper Bounds
+ * ub-name INTEGER ::= 32768
+ * ub-common-name INTEGER ::= 64
+ * ub-locality-name INTEGER ::= 128
+ * ub-state-name INTEGER ::= 128
+ * ub-organization-name INTEGER ::= 64
+ * ub-organizational-unit-name INTEGER ::= 64
+ * ub-title INTEGER ::= 64
+ * ub-serial-number INTEGER ::= 64
+ * ub-match INTEGER ::= 128
+ * ub-emailaddress-length INTEGER ::= 255
+ * ub-common-name-length INTEGER ::= 64
+ * ub-country-name-alpha-length INTEGER ::= 2
+ * ub-country-name-numeric-length INTEGER ::= 3
+ * ub-domain-defined-attributes INTEGER ::= 4
+ * ub-domain-defined-attribute-type-length INTEGER ::= 8
+ * ub-domain-defined-attribute-value-length INTEGER ::= 128
+ * ub-domain-name-length INTEGER ::= 16
+ * ub-extension-attributes INTEGER ::= 256
+ * ub-e163-4-number-length INTEGER ::= 15
+ * ub-e163-4-sub-address-length INTEGER ::= 40
+ * ub-generation-qualifier-length INTEGER ::= 3
+ * ub-given-name-length INTEGER ::= 16
+ * ub-initials-length INTEGER ::= 5
+ * ub-integer-options INTEGER ::= 256
+ * ub-numeric-user-id-length INTEGER ::= 32
+ * ub-organization-name-length INTEGER ::= 64
+ * ub-organizational-unit-name-length INTEGER ::= 32
+ * ub-organizational-units INTEGER ::= 4
+ * ub-pds-name-length INTEGER ::= 16
+ * ub-pds-parameter-length INTEGER ::= 30
+ * ub-pds-physical-address-lines INTEGER ::= 6
+ * ub-postal-code-length INTEGER ::= 16
+ * ub-pseudonym INTEGER ::= 128
+ * ub-surname-length INTEGER ::= 40
+ * ub-terminal-id-length INTEGER ::= 24
+ * ub-unformatted-address-length INTEGER ::= 180
+ * ub-x121-address-length INTEGER ::= 16
+ *
+ * -- Note - upper bounds on string types, such as TeletexString, are
+ * -- measured in characters.  Excepting PrintableString or IA5String, a
+ * -- significantly greater number of octets will be required to hold
+ * -- such a value.  As a minimum, 16 octets, or twice the specified
+ * -- upper bound, whichever is the larger, should be allowed for
+ * -- TeletexString.  For UTF8String or UniversalString at least four
+ * -- times the upper bound should be allowed.
+ *)
+
